FreydSSA/Ctx/Label/Perm.lean
@@ -7,6 +7,54 @@ inductive LCtx.LPerm : LCtx ν κ α → LCtx ν κ α → Prop
   | swap (ℓ ℓ') (L) : ℓ.name ≠ ℓ'.name -> LPerm (ℓ::ℓ'::L) (ℓ'::ℓ::L)
   | trans : LPerm Γ Δ → LPerm Δ Ξ → LPerm Γ Ξ
 
+theorem LCtx.LPerm.perm {L K : LCtx ν κ α} (h : L.LPerm K) : L.Perm K := by
+  induction h <;> constructor <;> assumption
+
+theorem LCtx.perm_nodup_iff {L K : LCtx ν κ α} (h : L.Perm K) : L.Nodup ↔ K.Nodup := by
+  apply List.Perm.nodup_iff
+  apply List.Perm.map
+  exact h
+
+theorem LCtx.Nodup.of_perm {L K : LCtx ν κ α} (h : L.Perm K)  (h' : L.Nodup) : K.Nodup
+  := (perm_nodup_iff h).mp h'
+
+theorem LCtx.Nodup.of_lperm {L K : LCtx ν κ α} (h : L.LPerm K)  (h' : L.Nodup)
+  : K.Nodup
+  := h'.of_perm h.perm
+
+theorem LCtx.Nodup.lperm {L K : LCtx ν κ α} (h : L.Nodup) (h' : L.Perm K) : L.LPerm K
+  := by
+  induction h' with
+  | nil => exact LPerm.nil
+  | cons v _ I => exact LPerm.cons (I h.tail)
+  | swap v v' I => exact LPerm.swap _ _ _ (λh' => h.not_mem (by simp [h']))
+  | trans l _ Il Ir => exact LPerm.trans (Il h) (Ir (h.of_perm l))
+
+theorem LCtx.Nodup.lperm_iff {L K : LCtx ν κ α} (h: L.Nodup) : L.LPerm K ↔ L.Perm K :=
+  ⟨LPerm.perm, h.lperm⟩
+
+theorem LCtx.Fresh.perm {L K : LCtx ν κ α} (h : L.Fresh ℓ) (h' : L.Perm K) : K.Fresh ℓ
+  := by
+   apply of_not_mem
+   intro c
+   apply h.not_mem
+   apply (h'.map Label.name).mem_iff.mpr c
+
+-- In this case, we simply have _pointwise_ comparability, probably, or smt...
+-- theorem LCtx.Comp.perm_eq {L K : LCtx ν κ α} (h : L.Comp K) (h' : L.Perm K) : L = K := by
+--   cases h with | mk base wl wr =>
+--   induction wl generalizing K with
+--   | nil => cases wr; rfl
+--   | cons hℓ _ I => cases wr with
+--     | cons hℓ' wr =>
+
+--       cases I ((List.perm_cons _).mp sorry) wr
+--       rfl
+--     | skip hvr wr => exact ((hvr.perm h'.symm).head rfl).elim
+--   | skip hvl _ I => cases wr with
+--     | cons vr wr => exact ((hvl.perm h').head rfl).elim
+--     | skip hvr wr => exact I h' wr
+
 structure Label.TPerm (ℓ : Label ν κ α) (ℓ' : Label ν κ α) :=
   name : ℓ.name = ℓ'.name
   param : ℓ.param = ℓ'.param
