FreydSSA/Ctx/Var/Perm.lean
@@ -20,6 +20,27 @@ theorem Ctx.TPerm.symm {Γ Δ : Ctx ν α} (h : Γ.TPerm Δ) : Δ.TPerm Γ := by
   | trans _ _ Il Ir => exact trans Ir Il
   | _ => constructor <;> assumption
 
+theorem Ctx.perm_nodup_iff {Γ Δ : Ctx ν α} (h : Γ.Perm Δ) : Γ.Nodup ↔ Δ.Nodup := by
+  apply List.Perm.nodup_iff
+  apply List.Perm.map
+  exact h
+
+theorem Ctx.Nodup.of_perm {Γ Δ : Ctx ν α} (h : Γ.Perm Δ)  (h' : Γ.Nodup) : Δ.Nodup
+  := (perm_nodup_iff h).mp h'
+
+theorem Ctx.Nodup.of_tperm {Γ Δ : Ctx ν α} (h : Γ.TPerm Δ) (h' : Γ.Nodup) : Δ.Nodup
+  := h'.of_perm h.perm
+
+theorem Ctx.Nodup.tperm {Γ Δ : Ctx ν α} (h : Γ.Nodup) (h' : Γ.Perm Δ) : Γ.TPerm Δ := by
+  induction h' with
+  | nil => exact TPerm.nil
+  | cons v _ I => exact TPerm.cons (I h.tail)
+  | swap v v' I => exact TPerm.swap _ _ _ (λh' => h.not_mem (by simp [h']))
+  | trans l _ Il Ir => exact TPerm.trans (Il h) (Ir (h.of_perm l))
+
+theorem Ctx.Nodup.tperm_iff {Γ Δ : Ctx ν α} (h: Γ.Nodup) : Γ.TPerm Δ ↔ Γ.Perm Δ :=
+  ⟨Ctx.TPerm.perm, h.tperm⟩
+
 -- theorem Ctx.TPerm.tail {Γ Δ : Ctx ν α} (h : TPerm Γ Δ) (h' : Γ.head? = Δ.head?)
 --   : TPerm Γ.tail Δ.tail := by
 --   induction Γ generalizing Δ with
@@ -31,15 +52,22 @@ theorem Ctx.TPerm.symm {Γ Δ : Ctx ν α} (h : Γ.TPerm Δ) : Δ.TPerm Γ := by
 -- theorem Ctx.TPerm.uncons {v : Var ν α} {Γ Δ : Ctx ν α} (h : TPerm (v::Γ) (v::Δ))
 --   : TPerm Γ Δ := h.tail rfl
 
--- theorem Ctx.TPerm.comp {Γ Δ : Ctx ν α} (h : Γ.TPerm Δ) (h' : Γ.Comp Δ) : Γ = Δ := by
---   cases h' with | mk base wl wr =>
---   induction wl generalizing Δ with
---   | nil => cases wr; rfl
---   | cons vl wl I => cases wr with
---     | cons _ wr =>
---       cases I h.uncons wr
---       rfl
---     | skip hvr wr => sorry -- contradiction by perm...
---   | skip hvl wl I => cases wr with
---     | cons vr wr => sorry -- contradiction by perm...
---     | skip hvr wr => exact I h wr
+theorem Ctx.Fresh.perm {Γ Δ : Ctx ν α} (h : Γ.Fresh v) (h' : Γ.Perm Δ) : Δ.Fresh v
+  := by
+   apply of_not_mem_names
+   intro c
+   apply h.not_mem_names
+   apply (h'.map Var.name).mem_iff.mpr c
+
+theorem Ctx.Comp.perm_eq {Γ Δ : Ctx ν α} (h : Γ.Comp Δ) (h' : Γ.Perm Δ) : Γ = Δ := by
+  cases h with | mk base wl wr =>
+  induction wl generalizing Δ with
+  | nil => cases wr; rfl
+  | cons vl _ I => cases wr with
+    | cons _ wr =>
+      cases I ((List.perm_cons _).mp h') wr
+      rfl
+    | skip hvr wr => exact ((hvr.perm h'.symm).head rfl).elim
+  | skip hvl _ I => cases wr with
+    | cons vr wr => exact ((hvl.perm h').head rfl).elim
+    | skip hvr wr => exact I h' wr
